src/riot/RIoT.Core.fst
@@ -21,6 +21,7 @@ open X509
 open RIoT.X509
 open RIoT.Base
 open RIoT.Declassify
+open RIoT.Helpers
 open RIoT.Spec
 open RIoT.Impl
 
@@ -72,7 +73,7 @@ let riot
    (* Pre: `aliasKeyCRT_buf` has exact size to write AliasKeyCRT *)
    v aliasKeyCRT_len == length_of_AliasKeyCRT (len_of_AliasKeyTBS aliasKeyTBS_template_len version)
    )
-   (ensures fun h0 _ h1 -> True /\
+   (ensures fun h0 _ h1 ->
     (* Post: Modifies *)
      B.(modifies (loc_buffer aliasKeyCRT_buf `loc_union` loc_buffer aliasKey_pub `loc_union` loc_buffer aliasKey_priv) h0 h1) /\
     (* Post: AliasKey *)
@@ -80,29 +81,29 @@ let riot
      (B.as_seq h1 aliasKey_priv <: lbytes_sec 32)) == derive_AliasKey_spec
                                                         (B.as_seq h0 cdi)
                                                         (B.as_seq h0 fwid)
-                                                        aliasKey_label_len                                                        (B.as_seq h0 aliasKey_label) /\
-    // (* Post: AliasKeyCRT *)
-    // (let deviceID_pub_seq, deviceID_priv_seq = derive_DeviceID_spec
-    //                                              (B.as_seq h0 cdi)
-    //                                              (deviceID_label_len)
-    //                                              (B.as_seq h0 deviceID_label) in
-    //  let aliasKeyTBS: aliasKeyTBS_t_inbound aliasKeyTBS_template_len = create_aliasKeyTBS_spec
-    //                                                                      (aliasKeyTBS_template_len)
-    //                                                                      (B.as_seq h0 aliasKeyTBS_template)
-    //                                                                      (version)
-    //                                                                      (B.as_seq h0 fwid)
-    //                                                                      (deviceID_pub_seq)
-    //                                                                      (B.as_seq h1 aliasKey_pub)
-    //                                                                      in
-    //  let aliasKeyTBS_seq = serialize_aliasKeyTBS_sequence_TLV aliasKeyTBS_template_len `serialize` aliasKeyTBS in
-    //  let aliasKeyTBS_len = len_of_AliasKeyTBS aliasKeyTBS_template_len version in
-    //  (* Prf *) lemma_serialize_aliasKeyTBS_sequence_TLV_size_exact aliasKeyTBS_template_len aliasKeyTBS;
-    // (let aliasKeyCRT: aliasKeyCRT_t_inbound aliasKeyTBS_len = sign_and_finalize_aliasKeyCRT_spec
-    //                                                             (deviceID_priv_seq)
-    //                                                             (aliasKeyTBS_len)
-    //                                                             (aliasKeyTBS_seq) in
-    //  B.as_seq h1 aliasKeyCRT_buf == serialize_aliasKeyCRT_sequence_TLV aliasKeyTBS_len `serialize` aliasKeyCRT))
-     True)
+                                                        aliasKey_label_len
+                                                        (B.as_seq h0 aliasKey_label) /\
+    (* Post: AliasKeyCRT *)
+    (let deviceID_pub_seq, deviceID_priv_seq = derive_DeviceID_spec
+                                                 (B.as_seq h0 cdi)
+                                                 (deviceID_label_len)
+                                                 (B.as_seq h0 deviceID_label) in
+     let aliasKeyTBS: aliasKeyTBS_t_inbound aliasKeyTBS_template_len = create_aliasKeyTBS_spec
+                                                                         (aliasKeyTBS_template_len)
+                                                                         (B.as_seq h0 aliasKeyTBS_template)
+                                                                         (version)
+                                                                         (B.as_seq h0 fwid)
+                                                                         (deviceID_pub_seq)
+                                                                         (B.as_seq h1 aliasKey_pub)
+                                                                         in
+     let aliasKeyTBS_seq = serialize_aliasKeyTBS_sequence_TLV aliasKeyTBS_template_len `serialize` aliasKeyTBS in
+     let aliasKeyTBS_len = len_of_AliasKeyTBS aliasKeyTBS_template_len version in
+     (* Prf *) lemma_serialize_aliasKeyTBS_sequence_TLV_size_exact aliasKeyTBS_template_len aliasKeyTBS;
+    (let aliasKeyCRT: aliasKeyCRT_t_inbound aliasKeyTBS_len = sign_and_finalize_aliasKeyCRT_spec
+                                                                (deviceID_priv_seq)
+                                                                (aliasKeyTBS_len)
+                                                                (aliasKeyTBS_seq) in
+     B.as_seq h1 aliasKeyCRT_buf == serialize_aliasKeyCRT_sequence_TLV aliasKeyTBS_len `serialize` aliasKeyCRT)))
 =
  HST.push_frame ();
 
@@ -154,6 +155,8 @@ let riot
   HST.pop_frame()
 #pop-options
 
+open RIoT.Helpers
+
 let template_len: size_t = 175ul
 
 unfold noextract inline_for_extraction
@@ -161,6 +164,7 @@ let template_list: List.llist byte_pub (v template_len)
 = [@inline_let]let l = [0xA0uy; 0x03uy; 0x02uy; 0x01uy; 0x02uy; 0x02uy; 0x01uy; 0x00uy; 0x30uy; 0x0Duy; 0x06uy; 0x09uy; 0x2Auy; 0x86uy; 0x48uy; 0x86uy; 0xF7uy; 0x0Duy; 0x01uy; 0x01uy; 0x0Duy; 0x05uy; 0x00uy; 0x30uy; 0x3Auy; 0x31uy; 0x0Buy; 0x30uy; 0x09uy; 0x06uy; 0x03uy; 0x55uy; 0x04uy; 0x06uy; 0x13uy; 0x02uy; 0x75uy; 0x73uy; 0x31uy; 0x0Duy; 0x30uy; 0x0Buy; 0x06uy; 0x03uy; 0x55uy; 0x04uy; 0x08uy; 0x0Cuy; 0x04uy; 0x74uy; 0x65uy; 0x73uy; 0x74uy; 0x31uy; 0x0Duy; 0x30uy; 0x0Buy; 0x06uy; 0x03uy; 0x55uy; 0x04uy; 0x0Auy; 0x0Cuy; 0x04uy; 0x74uy; 0x65uy; 0x73uy; 0x74uy; 0x31uy; 0x0Duy; 0x30uy; 0x0Buy; 0x06uy; 0x03uy; 0x55uy; 0x04uy; 0x03uy; 0x0Cuy; 0x04uy; 0x74uy; 0x65uy; 0x73uy; 0x74uy; 0x30uy; 0x1Euy; 0x17uy; 0x0Duy; 0x32uy; 0x30uy; 0x30uy; 0x36uy; 0x32uy; 0x35uy; 0x30uy; 0x32uy; 0x35uy; 0x37uy; 0x30uy; 0x32uy; 0x5Auy; 0x17uy; 0x0Duy; 0x32uy; 0x31uy; 0x30uy; 0x36uy; 0x32uy; 0x35uy; 0x30uy; 0x32uy; 0x35uy; 0x37uy; 0x30uy; 0x32uy; 0x5Auy; 0x30uy; 0x3Auy; 0x31uy; 0x0Buy; 0x30uy; 0x09uy; 0x06uy; 0x03uy; 0x55uy; 0x04uy; 0x06uy; 0x13uy; 0x02uy; 0x75uy; 0x73uy; 0x31uy; 0x0Duy; 0x30uy; 0x0Buy; 0x06uy; 0x03uy; 0x55uy; 0x04uy; 0x08uy; 0x0Cuy; 0x04uy; 0x74uy; 0x65uy; 0x73uy; 0x74uy; 0x31uy; 0x0Duy; 0x30uy; 0x0Buy; 0x06uy; 0x03uy; 0x55uy; 0x04uy; 0x0Auy; 0x0Cuy; 0x04uy; 0x74uy; 0x65uy; 0x73uy; 0x74uy; 0x31uy; 0x0Duy; 0x30uy; 0x0Buy; 0x06uy; 0x03uy; 0x55uy; 0x04uy; 0x03uy; 0x0Cuy; 0x04uy; 0x74uy; 0x65uy; 0x73uy; 0x74uy] in
   assert_norm (List.length l == v template_len);
   l
+
 
 #restart-solver
 #push-options "--query_stats --z3rlimit 1024 --fuel 0 --ifuel 0"
@@ -216,6 +220,10 @@ let main ()
   printf "AliasKey Public  Key: %xuy \n" 32ul aliasKey_pub  done;
   printf "AliasKey Private Key: %xuy \n" 32ul aliasKey_priv_pub done;
   printf "AliasKey Certificate: %xuy \n" aliasKeyCRT_len aliasKeyCRT_buf done;
+
+  write_out "AliasKeyPublicKey.hex" aliasKey_pub 32ul;
+  write_out "AliasKeyPrivateKey.hex" aliasKey_priv_pub 32ul;
+  write_out "AliasKeyCrt.hex" aliasKeyCRT_buf aliasKeyCRT_len;
 
   HST.pop_frame ();
   C.EXIT_SUCCESS
