src/riot/RIoT.Helpers.fsti
@@ -1,0 +1,29 @@
+module RIoT.Helpers
+
+open FStar.Char
+open FStar.String
+
+open LowStar.Printf
+open LowStar.Comment
+open LowStar.Failure
+
+module HS = FStar.HyperStack
+module HST = FStar.HyperStack.ST
+module MB = LowStar.Monotonic.Buffer
+module B = LowStar.Buffer
+module C = C
+
+open FStar.Integers
+
+val write_out
+  (filename: string)
+  (content: B.buffer uint_8)
+  (len: uint_32)
+: HST.Stack unit
+  (requires fun h ->
+    B.live h content /\
+    B.length content >= v len)
+  (ensures fun h0 _ h1 ->
+    B.live h1 content /\
+    B.modifies B.loc_none h0 h1)
+
