src/riot/asn1/ASN1.Low.Tag.fst
@@ -28,7 +28,7 @@ let encode_asn1_tag
   | INTEGER      -> 0x02uy
   | BIT_STRING   -> 0x03uy
   | OCTET_STRING -> 0x04uy
-  | NULL         -> 0x05uy
+  | ASN1_NULL         -> 0x05uy
   | OID          -> 0x06uy
   | SEQUENCE     -> 0x30uy
   | CUSTOM_TAG tag_class tag_form tag_value -> ( let b_tag_class = match tag_class with
