src/riot/asn1/ASN1.Low.Value.OID.fst
@@ -41,20 +41,20 @@ module G = FStar.Ghost
 // }
 
 (* ZT: Noramlize them here instead of mark OID lists as unfold and normalize them everywhere. *)
-let oid_RIOT_as_buffer                     = IB.igcmalloc_of_list HS.root (normalize_term (oid_RIOT))
-let oid_AT_CN_as_buffer                    = IB.igcmalloc_of_list HS.root (normalize_term (oid_AT_CN))
-let oid_AT_COUNTRY_as_buffer               = IB.igcmalloc_of_list HS.root (normalize_term (oid_AT_COUNTRY))
-let oid_AT_ORGANIZATION_as_buffer          = IB.igcmalloc_of_list HS.root (normalize_term (oid_AT_ORGANIZATION))
-let oid_CLIENT_AUTH_as_buffer              = IB.igcmalloc_of_list HS.root (normalize_term (oid_CLIENT_AUTH))
-let oid_AUTHORITY_KEY_IDENTIFIER_as_buffer = IB.igcmalloc_of_list HS.root (normalize_term (oid_AUTHORITY_KEY_IDENTIFIER))
-let oid_KEY_USAGE_as_buffer                = IB.igcmalloc_of_list HS.root (normalize_term (oid_KEY_USAGE))
-let oid_EXTENDED_KEY_USAGE_as_buffer       = IB.igcmalloc_of_list HS.root (normalize_term (oid_EXTENDED_KEY_USAGE))
-let oid_BASIC_CONSTRAINTS_as_buffer        = IB.igcmalloc_of_list HS.root (normalize_term (oid_BASIC_CONSTRAINTS))
-let oid_EC_ALG_UNRESTRICTED_as_buffer      = IB.igcmalloc_of_list HS.root (normalize_term (oid_EC_ALG_UNRESTRICTED))
-let oid_EC_GRP_SECP256R1_as_buffer         = IB.igcmalloc_of_list HS.root (normalize_term (oid_EC_GRP_SECP256R1))
-let oid_DIGEST_ALG_SHA256_as_buffer        = IB.igcmalloc_of_list HS.root (normalize_term (oid_DIGEST_ALG_SHA256))
-let oid_ED25519_as_bufffer                 = IB.igcmalloc_of_list HS.root (normalize_term (oid_ED25519))
-let oid_X25519_as_bufffer                  = IB.igcmalloc_of_list HS.root (normalize_term (oid_X25519))
+let oid_RIOT_as_buffer                     = IB.igcmalloc_of_list HS.root (oid_RIOT)
+let oid_AT_CN_as_buffer                    = IB.igcmalloc_of_list HS.root (oid_AT_CN)
+let oid_AT_COUNTRY_as_buffer               = IB.igcmalloc_of_list HS.root (oid_AT_COUNTRY)
+let oid_AT_ORGANIZATION_as_buffer          = IB.igcmalloc_of_list HS.root (oid_AT_ORGANIZATION)
+let oid_CLIENT_AUTH_as_buffer              = IB.igcmalloc_of_list HS.root (oid_CLIENT_AUTH)
+let oid_AUTHORITY_KEY_IDENTIFIER_as_buffer = IB.igcmalloc_of_list HS.root (oid_AUTHORITY_KEY_IDENTIFIER)
+let oid_KEY_USAGE_as_buffer                = IB.igcmalloc_of_list HS.root (oid_KEY_USAGE)
+let oid_EXTENDED_KEY_USAGE_as_buffer       = IB.igcmalloc_of_list HS.root (oid_EXTENDED_KEY_USAGE)
+let oid_BASIC_CONSTRAINTS_as_buffer        = IB.igcmalloc_of_list HS.root (oid_BASIC_CONSTRAINTS)
+let oid_EC_ALG_UNRESTRICTED_as_buffer      = IB.igcmalloc_of_list HS.root (oid_EC_ALG_UNRESTRICTED)
+let oid_EC_GRP_SECP256R1_as_buffer         = IB.igcmalloc_of_list HS.root (oid_EC_GRP_SECP256R1)
+let oid_DIGEST_ALG_SHA256_as_buffer        = IB.igcmalloc_of_list HS.root (oid_DIGEST_ALG_SHA256)
+let oid_ED25519_as_bufffer                 = IB.igcmalloc_of_list HS.root (oid_ED25519)
+let oid_X25519_as_bufffer                  = IB.igcmalloc_of_list HS.root (oid_X25519)
 
 (* FIXME: A workaround
    To not extract any (total) seq, we split the `oid_buffer_t` into three
@@ -112,6 +112,7 @@ let seq_of_oid_buffer
                  Seq.length s == length_of_oid oid})
 = lemma_known_oids_as_seq_contains_oid_seq_of oid;
   oid_seq_of oid
+
 
 // #push-options "--z3rlimit 32"
 // inline_for_extraction
