src/riot/asn1/ASN1.Spec.Tag.fst
@@ -48,7 +48,7 @@ let synth_asn1_tag
   | 0x02uy -> INTEGER
   | 0x03uy -> BIT_STRING
   | 0x04uy -> OCTET_STRING
-  | 0x05uy -> NULL
+  | 0x05uy -> ASN1_NULL
   | 0x06uy -> OID
   | 0x30uy -> SEQUENCE
   | _      -> ( let tag_class = match b / 0b01000000uy <: byte with
@@ -71,7 +71,7 @@ let synth_asn1_tag_inverse
   | INTEGER      -> 0x02uy
   | BIT_STRING   -> 0x03uy
   | OCTET_STRING -> 0x04uy
-  | NULL         -> 0x05uy
+  | ASN1_NULL         -> 0x05uy
   | OID          -> 0x06uy
   | SEQUENCE     -> 0x30uy
   | CUSTOM_TAG tag_class tag_form tag_value -> ( let b_tag_class = match tag_class with
@@ -207,7 +207,7 @@ let filter_asn1_tag_of_type
 //   | INTEGER     , 0x02uy
 //   | BIT_STRING  , 0x03uy
 //   | OCTET_STRING, 0x04uy
-//   | NULL        , 0x05uy
+//   | ASN1_NULL        , 0x05uy
 //   | OID         , 0x06uy
 //   | SEQUENCE    , 0x30uy
 //   | CUSTOM_TAG _ _ _, _ -> b = (synth_asn1_tag_inverse a <: byte)
