src/riot/asn1/ASN1.Spec.Value.NULL.fst
@@ -1,0 +1,208 @@
+module ASN1.Spec.Value.NULL
+
+open ASN1.Spec.Base
+
+open ASN1.Base
+open ASN1.Spec.Tag
+open ASN1.Spec.Length
+
+(* NOTE: Read after `ASN1.Spec.Tag`, `ASN1.Spec.Length` *)
+(* NOTE: This module defines:
+         1) The ASN1 `ASN1_NULL` Value Parser and Serializer
+         2) The ASN1 `ASN1_NULL` TLV Parser and Serializer
+*)
+
+///////////////////////////////////////////////////////////////
+////  ASN1 `ASN1_NULL` Value Parser/Serializer
+///////////////////////////////////////////////////////////////
+
+noextract
+let parse_asn1_ASN1_NULL_kind = parse_ret_kind
+
+///
+/// ASN1 `ASN1_NULL` value parser parses nothing and returns `()`
+/// using the `parse_ret` combinator
+///
+noextract
+let parse_asn1_ASN1_NULL
+: parser parse_asn1_ASN1_NULL_kind (datatype_of_asn1_type ASN1_NULL)
+= parse_ret
+  (* v *) ()
+
+///
+/// ASN1 `ASN1_NULL` value parser serialize `()` to empty bytes
+/// using the `serialize_ret` combinator
+///
+noextract
+let serialize_asn1_ASN1_NULL
+: serializer parse_asn1_ASN1_NULL
+= serialize_ret
+  (* v *) ()
+  (*prf*) (fun n -> ())
+
+///
+/// Lemmas
+///
+
+/// Reveal the computation of serialize
+noextract
+let lemma_serialize_asn1_ASN1_NULL_unfold
+  (value: datatype_of_asn1_type ASN1_NULL)
+: Lemma (
+  serialize serialize_asn1_ASN1_NULL value == Seq.empty)
+= ()
+
+/// Reveal the size of a serialiaztion
+noextract
+let lemma_serialize_asn1_ASN1_NULL_size
+  (value: datatype_of_asn1_type ASN1_NULL)
+: Lemma (
+  Seq.length (serialize serialize_asn1_ASN1_NULL value) == 0)
+= parser_kind_prop_equiv parse_asn1_ASN1_NULL_kind parse_asn1_ASN1_NULL;
+  lemma_serialize_asn1_ASN1_NULL_unfold value
+
+///////////////////////////////////////////////////////////////
+////  ASN1 `ASN1_NULL` TLV Parser/Serializer
+///////////////////////////////////////////////////////////////
+
+/// Synthesize the TLV of a `ASN1_NULL` value
+noextract
+let synth_asn1_ASN1_NULL_TLV
+  (a: (the_asn1_tag ASN1_NULL * asn1_value_int32_of_type ASN1_NULL) * datatype_of_asn1_type ASN1_NULL)
+: GTot (datatype_of_asn1_type ASN1_NULL)
+= snd a
+
+/// Synthesize th `ASN1_NULL` value from a `ASN1_NULL` TLV
+noextract
+let synth_asn1_ASN1_NULL_TLV_inverse
+  (x: datatype_of_asn1_type ASN1_NULL)
+: GTot (a: ((the_asn1_tag ASN1_NULL * asn1_value_int32_of_type ASN1_NULL) * datatype_of_asn1_type ASN1_NULL){x == synth_asn1_ASN1_NULL_TLV a})
+= ((ASN1_NULL, 0ul), x)
+
+inline_for_extraction noextract
+let parse_asn1_ASN1_NULL_TLV_kind
+: parser_kind
+= strong_parser_kind 2 2 None
+
+///
+/// `ASN1_NULL` TLV parser
+///
+noextract
+let parse_asn1_ASN1_NULL_TLV
+: parser parse_asn1_ASN1_NULL_TLV_kind (datatype_of_asn1_type ASN1_NULL)
+= parse_asn1_tag_of_type ASN1_NULL
+  `nondep_then`
+  parse_asn1_length_of_type ASN1_NULL
+  `nondep_then`
+  parse_asn1_ASN1_NULL
+  `parse_synth`
+  synth_asn1_ASN1_NULL_TLV
+
+///
+/// `ASN1_NULL` TLV serialzier
+///
+noextract
+let serialize_asn1_ASN1_NULL_TLV
+: serializer parse_asn1_ASN1_NULL_TLV
+= serialize_synth
+  (* p1 *) (parse_asn1_tag_of_type ASN1_NULL
+            `nondep_then`
+            parse_asn1_length_of_type ASN1_NULL
+            `nondep_then`
+            parse_asn1_ASN1_NULL)
+  (* f2 *) (synth_asn1_ASN1_NULL_TLV)
+  (* s1 *) (serialize_asn1_tag_of_type ASN1_NULL
+            `serialize_nondep_then`
+            serialize_asn1_length_of_type ASN1_NULL
+            `serialize_nondep_then`
+            serialize_asn1_ASN1_NULL)
+  (* g1 *) (synth_asn1_ASN1_NULL_TLV_inverse)
+  (* Prf*) ()
+
+///
+/// Lemmas
+///
+
+/// Reveal the computation of parse
+noextract
+let lemma_parse_asn1_ASN1_NULL_TLV_unfold
+  (input_TLV: bytes)
+: Lemma (
+  parse parse_asn1_ASN1_NULL_TLV input_TLV ==
+ (match parse (parse_asn1_tag_of_type ASN1_NULL) input_TLV with
+  | None -> None
+  | Some (ASN1_NULL, consumed_T) ->
+    (let input_LV = Seq.slice input_TLV consumed_T (Seq.length input_TLV) in
+     match parse (parse_asn1_length_of_type ASN1_NULL) input_LV with
+     | None -> None
+     | Some (0ul, consumed_L) ->
+       (let input_V = Seq.slice input_LV consumed_L (Seq.length input_LV) in
+        match parse parse_asn1_ASN1_NULL input_V with
+        | None -> None
+        | Some (value, consumed_V) -> Some (value, (consumed_T + consumed_L + consumed_V <: consumed_length input_TLV)))))
+)
+= nondep_then_eq
+  (* p1 *) (parse_asn1_tag_of_type ASN1_NULL)
+  (* p2 *) (parse_asn1_length_of_type ASN1_NULL)
+  (* in *) (input_TLV);
+  nondep_then_eq
+  (* p1 *) (parse_asn1_tag_of_type ASN1_NULL
+            `nondep_then`
+            parse_asn1_length_of_type ASN1_NULL)
+  (* p2 *) (parse_asn1_ASN1_NULL)
+  (* in *) (input_TLV);
+  parse_synth_eq
+  (* p1 *) (parse_asn1_tag_of_type ASN1_NULL
+            `nondep_then`
+            parse_asn1_length_of_type ASN1_NULL
+            `nondep_then`
+            parse_asn1_ASN1_NULL)
+  (* f2 *) (synth_asn1_ASN1_NULL_TLV)
+  (* in *) (input_TLV)
+
+/// Reveal the computation of serialize
+noextract
+let lemma_serialize_asn1_ASN1_NULL_TLV_unfold
+  (value: datatype_of_asn1_type ASN1_NULL)
+: Lemma (
+  serialize serialize_asn1_ASN1_NULL_TLV value
+  `Seq.equal`
+ (serialize (serialize_asn1_tag_of_type ASN1_NULL) ASN1_NULL
+  `Seq.append`
+  serialize (serialize_asn1_length_of_type ASN1_NULL) 0ul
+  `Seq.append`
+  serialize serialize_asn1_ASN1_NULL value)
+)
+= serialize_nondep_then_eq
+  (* s1 *) (serialize_asn1_tag_of_type ASN1_NULL)
+  (* s2 *) (serialize_asn1_length_of_type ASN1_NULL)
+  (* in *) (ASN1_NULL, 0ul);
+  serialize_nondep_then_eq
+  (* s1 *) (serialize_asn1_tag_of_type ASN1_NULL
+            `serialize_nondep_then`
+            serialize_asn1_length_of_type ASN1_NULL)
+  (* s2 *) (serialize_asn1_ASN1_NULL)
+  (* in *) ((ASN1_NULL, 0ul), value);
+  serialize_synth_eq
+  (* p1 *) (parse_asn1_tag_of_type ASN1_NULL
+            `nondep_then`
+            parse_asn1_length_of_type ASN1_NULL
+            `nondep_then`
+            parse_asn1_ASN1_NULL)
+  (* f2 *) (synth_asn1_ASN1_NULL_TLV)
+  (* s1 *) (serialize_asn1_tag_of_type ASN1_NULL
+            `serialize_nondep_then`
+            serialize_asn1_length_of_type ASN1_NULL
+            `serialize_nondep_then`
+            serialize_asn1_ASN1_NULL)
+  (* g1 *) (synth_asn1_ASN1_NULL_TLV_inverse)
+  (* Prf*) ()
+  (* in *) (value)
+
+/// Reveal the length of a serialization
+noextract
+let lemma_serialize_asn1_ASN1_NULL_TLV_size
+  (value: datatype_of_asn1_type ASN1_NULL)
+: Lemma (
+  Seq.length (serialize serialize_asn1_ASN1_NULL_TLV value) == 2)
+= lemma_serialize_asn1_ASN1_NULL_TLV_unfold value
